code/bignum/Hacl.Bignum.Lib.fst
@@ -94,16 +94,16 @@ let cswap2_st #t len bit b1 b2 =
 
 
 inline_for_extraction noextract
-val bn_leading_zero_index:
+val bn_get_top_index:
     #t:limb_t
   -> len:size_t{0 < v len}
   -> b:lbignum t len ->
   Stack (limb t)
   (requires fun h -> live h b)
   (ensures  fun h0 r h1 -> modifies0 h0 h1 /\
-    v r == S.bn_leading_zero_index (as_seq h0 b))
+    v r == S.bn_get_top_index (as_seq h0 b))
 
-let bn_leading_zero_index #t len b =
+let bn_get_top_index #t len b =
   push_frame ();
   let priv = create 1ul (uint #t 0) in
 
@@ -111,18 +111,18 @@ let bn_leading_zero_index #t len b =
   [@ inline_let]
   let refl h i = v (LSeq.index (as_seq h priv) 0) in
   [@ inline_let]
-  let spec h0 = S.bn_leading_zero_index_f (as_seq h0 b) in
+  let spec h0 = S.bn_get_top_index_f (as_seq h0 b) in
 
   [@ inline_let]
   let inv h (i:nat{i <= v len}) =
     modifies1 priv h0 h /\
     live h priv /\ live h b /\ disjoint priv b /\
-    refl h i == Loops.repeat_gen i (S.bn_leading_zero_index_t (v len)) (spec h0) (refl h0 0) in
+    refl h i == Loops.repeat_gen i (S.bn_get_top_index_t (v len)) (spec h0) (refl h0 0) in
 
-  Loops.eq_repeat_gen0 (v len) (S.bn_leading_zero_index_t (v len)) (spec h0) (refl h0 0);
+  Loops.eq_repeat_gen0 (v len) (S.bn_get_top_index_t (v len)) (spec h0) (refl h0 0);
   Lib.Loops.for 0ul len inv
   (fun i ->
-    Loops.unfold_repeat_gen (v len) (S.bn_leading_zero_index_t (v len)) (spec h0) (refl h0 0) (v i);
+    Loops.unfold_repeat_gen (v len) (S.bn_get_top_index_t (v len)) (spec h0) (refl h0 0) (v i);
     let mask = eq_mask b.(i) (zeros t SEC) in
     let h1 = ST.get () in
     priv.(0ul) <- mask_select mask priv.(0ul) (size_to_limb i);
@@ -130,56 +130,3 @@ let bn_leading_zero_index #t len b =
   let res = priv.(0ul) in
   pop_frame ();
   res
-
-
-inline_for_extraction noextract
-val limb_leading_zero_index: #t:limb_t -> a:limb t ->
-  Stack (limb t)
-  (requires fun h -> True)
-  (ensures  fun h0 r h1 -> modifies0 h0 h1 /\
-    v r == S.limb_leading_zero_index a)
-
-let limb_leading_zero_index #t a =
-  push_frame ();
-  let priv = create 1ul (uint #t 0) in
-
-  let h0 = ST.get () in
-  [@ inline_let]
-  let refl h i = v (LSeq.index (as_seq h priv) 0) in
-  [@ inline_let]
-  let spec h0 = S.limb_leading_zero_index_f a in
-
-  [@ inline_let]
-  let inv h (i:nat{i <= bits t}) =
-    modifies1 priv h0 h /\ live h priv /\
-    refl h i == Loops.repeat_gen i (S.limb_leading_zero_index_t t) (spec h0) (refl h0 0) in
-
-  Loops.eq_repeat_gen0 (bits t) (S.limb_leading_zero_index_t t) (spec h0) (refl h0 0);
-  Lib.Loops.for 0ul (size (bits t)) inv
-  (fun i ->
-    Loops.unfold_repeat_gen (bits t) (S.limb_leading_zero_index_t t) (spec h0) (refl h0 0) (v i);
-    let bit_i = (a >>. i) &. uint #t 1 in
-    let mask = eq_mask bit_i (uint #t 1) in
-    let h1 = ST.get () in
-    priv.(0ul) <- mask_select mask (size_to_limb i) priv.(0ul);
-    mask_select_lemma mask (size_to_limb i) (LSeq.index (as_seq h1 priv) 0));
-  let res = priv.(0ul) in
-  pop_frame ();
-  res
-
-
-inline_for_extraction noextract
-val bn_get_num_bits:
-    #t:limb_t
-  -> len:size_t{0 < v len /\ bits t * v len <= max_size_t}
-  -> b:lbignum t len ->
-  Stack (limb t)
-  (requires fun h -> live h b)
-  (ensures  fun h0 r h1 -> modifies0 h0 h1 /\
-    v r == S.bn_get_num_bits (as_seq h0 b))
-
-let bn_get_num_bits #t len b =
-  //TODO: call `limb_leading_zero_index` for each limb
-  let ind = bn_leading_zero_index len b in
-  let bs = limb_leading_zero_index b.(Lib.RawIntTypes.(size_from_UInt32 (u32_to_UInt32 (to_u32 ind)))) in
-  uint #t (bits t) *! ind +! bs
