code/bignum/Hacl.Bignum.ModInv.fst
@@ -22,7 +22,8 @@ module BM = Hacl.Bignum.Montgomery
 
 inline_for_extraction noextract
 let bn_mod_inv_prime_st (t:limb_t) (len:BN.meta_len t) =
-    n:lbignum t len
+    nBits:size_t{v nBits / bits t < v len}
+  -> n:lbignum t len
   -> a:lbignum t len
   -> res:lbignum t len ->
   Stack unit
@@ -30,17 +31,17 @@ let bn_mod_inv_prime_st (t:limb_t) (len:BN.meta_len t) =
     live h n /\ live h a /\ live h res /\
     disjoint res n /\ disjoint res a /\ disjoint n a)
   (ensures  fun h0 r h1 -> modifies (loc res) h0 h1 /\
-    as_seq h1 res == S.bn_mod_inv_prime (as_seq h0 n) (as_seq h0 a))
+    as_seq h1 res == S.bn_mod_inv_prime (v nBits) (as_seq h0 n) (as_seq h0 a))
 
 
 inline_for_extraction noextract
 val bn_mod_inv_prime: #t:limb_t -> k:BE.exp t -> bn_mod_inv_prime_st t k.BE.mont.BM.bn.BN.len
-let bn_mod_inv_prime #t k n a res =
+let bn_mod_inv_prime #t k nBits n a res =
   [@inline_let] let len = k.BE.mont.BM.bn.BN.len in
   push_frame ();
   let b2 = create 1ul (uint #t #SEC 2) in
   let n2 = create len (uint #t #SEC 0) in
   let c = BN.bn_sub len n 1ul b2 n2 in
 
-  k.BE.mod_exp n a (size (bits t) *! len) n2 res;
+  k.BE.mod_exp nBits n a (size (bits t) *! len) n2 res;
   pop_frame ()
