code/bignum/Hacl.Bignum.SafeAPI.fst
@@ -13,6 +13,7 @@ module B = LowStar.Buffer
 module HS = FStar.HyperStack
 module LSeq = Lib.Sequence
 
+module BL = Hacl.Bignum.Lib
 module BB = Hacl.Bignum.Base
 module BN = Hacl.Bignum
 module BM = Hacl.Bignum.Montgomery
@@ -20,6 +21,7 @@ module BE = Hacl.Bignum.Exponentiation
 module BR = Hacl.Bignum.ModReduction
 module BC = Hacl.Bignum.Convert
 
+module SL = Hacl.Spec.Bignum.Lib
 module SD = Hacl.Spec.Bignum.Definitions
 module SR = Hacl.Spec.Bignum.ModReduction
 module SE = Hacl.Spec.Bignum.Exponentiation
@@ -75,20 +77,21 @@ let new_bn_from_bytes_be #t r len b =
 inline_for_extraction noextract
 let new_bn_precomp_r2_mod_n_st (t:limb_t) =
     r:HS.rid
-  -> nLen:size_t
-  -> n:lbignum t nLen ->
+  -> len:size_t
+  -> n:lbignum t len ->
   ST (B.buffer (limb t))
   (requires fun h -> live h n /\ ST.is_eternal_region r)
   (ensures  fun h0 res h1 ->
     B.(modifies loc_none h0 h1) /\
     not (B.g_is_null res) ==> (
-      0 < v nLen /\ 2 * bits t * v nLen <= max_size_t /\
+      0 < v len /\ 2 * bits t * v len <= max_size_t /\
       1 < bn_v h0 n /\ bn_v h0 n % 2 = 1 /\
-      B.len res == nLen /\
+      B.len res == len /\
       B.(fresh_loc (loc_buffer res) h0 h1) /\
       B.(loc_includes (loc_region_only false r) (loc_buffer res)) /\
-      as_seq h1 (res <: lbignum t nLen) == SM.bn_precomp_r2_mod_n (as_seq h0 n) /\
-      bn_v #t #nLen h1 res == pow2 (2 * bits t * v nLen) % bn_v h0 n))
+      as_seq h1 (res <: lbignum t len) ==
+	SM.bn_precomp_r2_mod_n (SL.bn_low_bound_bits #t #(v len) (as_seq h0 n)) (as_seq h0 n) /\
+      bn_v #t #len h1 res == pow2 (2 * bits t * v len) % bn_v h0 n))
 
 
 inline_for_extraction noextract
@@ -100,7 +103,7 @@ let new_bn_precomp_r2_mod_n #t r len n =
   then B.null
   else
     let is_valid_m = BM.bn_check_modulus n in
-    if not (Hacl.Bignum.Base.unsafe_bool_of_limb is_valid_m) then
+    if not (BB.unsafe_bool_of_limb is_valid_m) then
       B.null
     else
       let h0 = ST.get () in
@@ -114,10 +117,12 @@ let new_bn_precomp_r2_mod_n #t r len n =
 	let res: Lib.Buffer.buffer (limb t) = res in
 	assert (B.length res == FStar.UInt32.v len);
 	let res: lbignum t len = res in
-	BM.bn_precomp_r2_mod_n (BN.mk_runtime_bn t len) n res;
+	let nBits = size (bits t) *! BB.unsafe_size_from_limb (BL.bn_get_top_index len n) in
+	SL.bn_low_bound_bits_lemma #t #(v len) (as_seq h0 n);
+	BM.bn_precomp_r2_mod_n (BN.mk_runtime_bn t len) nBits n res;
 	let h2 = ST.get () in
 	B.(modifies_only_not_unused_in loc_none h0 h2);
-	SM.bn_precomp_r2_mod_n_lemma (as_seq h0 n);
+	SM.bn_precomp_r2_mod_n_lemma (v nBits) (as_seq h0 n);
 	res
 
 
@@ -147,14 +152,17 @@ let bn_mod_slow_safe #t k bn_check_bn_mod bn_mod_slow n a res =
   [@inline_let] let len = k.BM.bn.BN.len in
   let h0 = ST.get () in
   let is_valid_m = bn_check_bn_mod n a in
-  bn_mod_slow n a res;
+  let nBits = size (bits t) *! BB.unsafe_size_from_limb (BL.bn_get_top_index len n) in
+
+  bn_mod_slow nBits n a res;
   let h1 = ST.get () in
   mapT len res (logand is_valid_m) res;
   let h2 = ST.get () in
   SD.bn_mask_lemma (as_seq h1 res) is_valid_m;
 
   if BB.unsafe_bool_of_limb is_valid_m then begin
-    SR.bn_mod_slow_lemma (as_seq h0 n) (as_seq h0 a);
+    SL.bn_low_bound_bits_lemma #t #(v len) (as_seq h0 n);
+    SR.bn_mod_slow_lemma (v nBits) (as_seq h0 n) (as_seq h0 a);
     assert (bn_v h2 res == bn_v h0 a % bn_v h0 n) end;
   BB.unsafe_bool_of_limb is_valid_m
 
@@ -187,14 +195,17 @@ let bn_mod_exp_safe #t k bn_check_mod_exp bn_mod_exp n a bBits b res =
   [@inline_let] let len = k.BM.bn.BN.len in
   let h0 = ST.get () in
   let is_valid_m = bn_check_mod_exp n a bBits b in
-  bn_mod_exp n a bBits b res;
+  let nBits = size (bits t) *! BB.unsafe_size_from_limb (BL.bn_get_top_index len n) in
+
+  bn_mod_exp nBits n a bBits b res;
   let h1 = ST.get () in
   mapT len res (logand is_valid_m) res;
   let h2 = ST.get () in
   SD.bn_mask_lemma (as_seq h1 res) is_valid_m;
 
   if BB.unsafe_bool_of_limb is_valid_m then begin
-    SE.bn_mod_exp_lemma (v len) (as_seq h0 n) (as_seq h0 a) (v bBits) (as_seq h0 b);
+    SL.bn_low_bound_bits_lemma #t #(v len) (as_seq h0 n);
+    SE.bn_mod_exp_lemma (v len) (v nBits) (as_seq h0 n) (as_seq h0 a) (v bBits) (as_seq h0 b);
     assert (SE.bn_mod_exp_post (as_seq h0 n) (as_seq h0 a) (v bBits) (as_seq h0 b) (as_seq h2 res)) end;
   BB.unsafe_bool_of_limb is_valid_m
 
@@ -211,13 +222,16 @@ let bn_mod_exp_mont_ladder_safe #t k bn_check_mod_exp bn_mod_exp_mont_ladder n a
   [@inline_let] let len = k.BM.bn.BN.len in
   let h0 = ST.get () in
   let is_valid_m = bn_check_mod_exp n a bBits b in
-  bn_mod_exp_mont_ladder n a bBits b res;
+  let nBits = size (bits t) *! BB.unsafe_size_from_limb (BL.bn_get_top_index len n) in
+
+  bn_mod_exp_mont_ladder nBits n a bBits b res;
   let h1 = ST.get () in
   mapT len res (logand is_valid_m) res;
   let h2 = ST.get () in
   SD.bn_mask_lemma (as_seq h1 res) is_valid_m;
 
   if BB.unsafe_bool_of_limb is_valid_m then begin
-    SE.bn_mod_exp_mont_ladder_lemma (v len) (as_seq h0 n) (as_seq h0 a) (v bBits) (as_seq h0 b);
+    SL.bn_low_bound_bits_lemma #t #(v len) (as_seq h0 n);
+    SE.bn_mod_exp_mont_ladder_lemma (v len) (v nBits) (as_seq h0 n) (as_seq h0 a) (v bBits) (as_seq h0 b);
     assert (SE.bn_mod_exp_post (as_seq h0 n) (as_seq h0 a) (v bBits) (as_seq h0 b) (as_seq h1 res)) end;
   BB.unsafe_bool_of_limb is_valid_m
