code/bignum/Hacl.Spec.Bignum.Lib.fst
@@ -291,42 +291,39 @@ let cswap2_lemma #t #len bit b1 b2 =
   //eq_intro p2 (if v bit = 1 then b1 else b2);
   ()
 
-///
-///  bn_get_num_bits
-///
 
-let bn_leading_zero_index_t (len:size_nat) (i:nat{i <= len}) = x:nat{x < len}
+let bn_get_top_index_t (len:size_nat) (i:nat{i <= len}) = x:nat{x < len}
 
-val bn_leading_zero_index_f:
+val bn_get_top_index_f:
     #t:limb_t
   -> #len:size_nat
   -> b:lbignum t len
   -> i:nat{i < len}
-  -> priv:bn_leading_zero_index_t len i ->
-  bn_leading_zero_index_t len (i + 1)
+  -> priv:bn_get_top_index_t len i ->
+  bn_get_top_index_t len (i + 1)
 
-let bn_leading_zero_index_f #t #len b i priv =
+let bn_get_top_index_f #t #len b i priv =
   let mask = eq_mask b.[i] (zeros t SEC) in
   if v mask = 0 then i else priv
 
-val bn_leading_zero_index: #t:limb_t -> #len:size_pos -> b:lbignum t len -> res:size_nat{res < len}
-let bn_leading_zero_index #t #len b =
-  Loops.repeat_gen len (bn_leading_zero_index_t len) (bn_leading_zero_index_f #t #len b) 0
+val bn_get_top_index: #t:limb_t -> #len:size_pos -> b:lbignum t len -> res:size_nat{res < len}
+let bn_get_top_index #t #len b =
+  Loops.repeat_gen len (bn_get_top_index_t len) (bn_get_top_index_f #t #len b) 0
 
 
-val bn_leading_zero_index_lemma: #t:limb_t -> #len:size_pos -> b:lbignum t len ->
-  Lemma (let ind = bn_leading_zero_index #t #len b in
+val bn_get_top_index_lemma: #t:limb_t -> #len:size_pos -> b:lbignum t len ->
+  Lemma (let ind = bn_get_top_index #t #len b in
     ind < len /\ (ind > 0 ==> v b.[ind] <> 0) /\ (forall (k:nat{ind < k /\ k < len}). v b.[k] = 0))
 
-let bn_leading_zero_index_lemma #t #len b =
-  Loops.eq_repeat_gen0 len (bn_leading_zero_index_t len) (bn_leading_zero_index_f #t #len b) 0;
+let bn_get_top_index_lemma #t #len b =
+  Loops.eq_repeat_gen0 len (bn_get_top_index_t len) (bn_get_top_index_f #t #len b) 0;
   let res =
   Loops.repeati_inductive #size_nat len
   (fun i priv ->
-    priv == Loops.repeat_gen i (bn_leading_zero_index_t len) (bn_leading_zero_index_f #t #len b) 0 /\
+    priv == Loops.repeat_gen i (bn_get_top_index_t len) (bn_get_top_index_f #t #len b) 0 /\
     priv < len /\ (priv > 0 ==> v b.[priv] <> 0) /\ (forall (k:nat{priv < k /\ k < i}). v b.[k] = 0))
   (fun i priv ->
-    Loops.unfold_repeat_gen (i + 1) (bn_leading_zero_index_t len) (bn_leading_zero_index_f #t #len b) 0 i;
+    Loops.unfold_repeat_gen (i + 1) (bn_get_top_index_t len) (bn_get_top_index_f #t #len b) 0 i;
     let mask = eq_mask b.[i] (zeros t SEC) in
     eq_mask_lemma b.[i] (zeros t SEC);
     assert (if v mask = 0 then v b.[i] <> 0 else v b.[i] = 0);
@@ -335,13 +332,13 @@ let bn_leading_zero_index_lemma #t #len b =
   ()
 
 
-val bn_leading_zero_index_eval_lemma: #t:limb_t -> #len:size_pos -> b:lbignum t len -> ind:nat -> Lemma
+val bn_get_top_index_eval_lemma: #t:limb_t -> #len:size_pos -> b:lbignum t len -> ind:nat -> Lemma
   (requires
     ind < len /\ (ind > 0 ==> v b.[ind] <> 0) /\ (forall (k:nat{ind < k /\ k < len}). v b.[k] = 0))
   (ensures
     bn_v b == bn_v (slice b 0 ind) + pow2 (bits t * ind) * v b.[ind])
 
-let bn_leading_zero_index_eval_lemma #t #len b ind =
+let bn_get_top_index_eval_lemma #t #len b ind =
   let pbits = bits t in
   assert (forall (k:nat{ind < k /\ k < len}). v b.[k] = 0);
   bn_eval_split_i b (ind + 1);
@@ -355,327 +352,26 @@ let bn_leading_zero_index_eval_lemma #t #len b ind =
   assert (bn_v b == bn_v (slice b 0 ind) + pow2 (pbits * ind) * v b.[ind])
 
 
-
-let limb_leading_zero_index_t (t:limb_t) (i:nat{i <= bits t}) = x:size_nat{x < bits t}
-
-val limb_leading_zero_index_f:
+val bn_low_bound_bits:
     #t:limb_t
-  -> a:limb t
-  -> i:nat{i < bits t}
-  -> priv:limb_leading_zero_index_t t i ->
-  limb_leading_zero_index_t t (i + 1)
+  -> #len:size_pos{bits t * len <= max_size_t}
+  -> b:lbignum t len{0 < bn_v b} ->
+  res:size_nat{res / bits t < len}
 
-let limb_leading_zero_index_f #t a i priv =
-  if v (limb_get_ith_bit a i) = 1 then i else priv
-
-
-val limb_leading_zero_index: #t:limb_t -> a:limb t -> res:size_nat{res < bits t}
-let limb_leading_zero_index #t a =
-  Loops.repeat_gen (bits t) (limb_leading_zero_index_t t) (limb_leading_zero_index_f a) 0
+let bn_low_bound_bits #t #len b =
+  bits t * bn_get_top_index b
 
 
-val limb_leading_zero_index_lemma: #t:limb_t -> a:limb t ->
-  Lemma (let ind = limb_leading_zero_index a in
-    ind < bits t /\ (ind > 0 ==> v (limb_get_ith_bit a ind) = 1) /\
-    (forall (k:nat{ind < k /\ k < bits t}). v (limb_get_ith_bit a k) = 0))
+val bn_low_bound_bits_lemma: #t:limb_t -> #len:size_pos -> b:lbignum t len -> Lemma
+  (requires 1 < bn_v b /\ bits t * len <= max_size_t /\ bn_v b % 2 = 1)
+  (ensures  pow2 (bn_low_bound_bits b) < bn_v b)
 
-let limb_leading_zero_index_lemma #t a =
-  Loops.eq_repeat_gen0 (bits t) (limb_leading_zero_index_t t) (limb_leading_zero_index_f a) 0;
-  let res =
-  Loops.repeati_inductive #size_nat (bits t)
-  (fun i priv ->
-    priv == Loops.repeat_gen i (limb_leading_zero_index_t t) (limb_leading_zero_index_f a) 0 /\
-    priv < bits t /\ (priv > 0 ==> v (limb_get_ith_bit a priv) = 1) /\
-    (forall (k:nat{priv < k /\ k < i}). v (limb_get_ith_bit a k) = 0))
-  (fun i priv ->
-    Loops.unfold_repeat_gen (i + 1) (limb_leading_zero_index_t t) (limb_leading_zero_index_f a) 0 i;
-    limb_get_ith_bit_lemma a i;
-    let res = if v (limb_get_ith_bit a i) = 1 then i else priv in
-    res) 0 in
-  ()
-
-
-val limb_leading_zero_eval_lemma_aux: #t:limb_t -> a:limb t -> ind:nat{ind < bits t} -> j:nat{ind < j /\ j <= bits t} -> Lemma
-  (requires (forall (k:nat{ind < k /\ k < bits t}). v a / pow2 k % 2 = 0))
-  (ensures  v a / pow2 j = 0)
-  (decreases (bits t - j))
-
-let rec limb_leading_zero_eval_lemma_aux #t a ind j =
-  if j = bits t then ()
-  else begin
-    limb_leading_zero_eval_lemma_aux a ind (j + 1);
-    assert (v a / pow2 (j + 1) = 0);
-    calc (==) {
-      v a / pow2 j;
-      (==) { Math.Lemmas.euclidean_division_definition (v a / pow2 j) 2 }
-      (v a / pow2 j) / 2 * 2 + v a / pow2 j % 2;
-      (==) { assert_norm (pow2 1 = 2); Math.Lemmas.division_multiplication_lemma (v a) (pow2 j) (pow2 1) }
-      (v a / (pow2 j * pow2 1)) * 2 + v a / pow2 j % 2;
-      (==) { Math.Lemmas.pow2_plus j 1 }
-      (v a / pow2 (j + 1)) * 2 + v a / pow2 j % 2;
-      (==) { }
-      0;
-      }; () end
-
-
-val limb_leading_zero_index_eval_lemma: #t:limb_t -> a:limb t{v a > 0} -> ind:nat -> Lemma
-  (requires
-    ind < bits t /\ (ind > 0 ==> v (limb_get_ith_bit a ind) = 1) /\
-    (forall (k:nat{ind < k /\ k < bits t}). v (limb_get_ith_bit a k) = 0))
-  (ensures
-    pow2 ind <= v a /\ v a < pow2 (ind + 1))
-
-let limb_leading_zero_index_eval_lemma #t a ind =
-  let aux (k:nat{ind < k /\ k < bits t}) : Lemma (v a / pow2 k % 2 = 0) =
-    assert (v (limb_get_ith_bit a k) = 0);
-    limb_get_ith_bit_lemma a k;
-    assert (v a / pow2 k % 2 = 0);
-    () in
-  Classical.forall_intro aux;
-  assert (forall (k:nat{ind < k /\ k < bits t}). v a / pow2 k % 2 = 0);
-
-  limb_leading_zero_eval_lemma_aux a ind (ind + 1);
-  assert (v a / pow2 (ind + 1) = 0);
-
-  if ind = 0 then begin
-    assert_norm (pow2 0 = 1);
-    assert_norm (pow2 1 = 2);
-    assert (v a = 1) end
-  else begin
-    calc (==) {
-      v a / pow2 ind;
-      (==) { Math.Lemmas.euclidean_division_definition (v a / pow2 ind) 2 }
-      (v a / pow2 ind) / 2 * 2 + v a / pow2 ind % 2;
-      (==) { assert_norm (pow2 1 = 2);
-	Math.Lemmas.division_multiplication_lemma (v a) (pow2 ind) (pow2 1) }
-      (v a / (pow2 ind * pow2 1)) * 2 + v a / pow2 ind % 2;
-      (==) { Math.Lemmas.pow2_plus ind 1 }
-      (v a / pow2 (ind + 1)) * 2 + v a / pow2 ind % 2;
-      (==) { }
-      v a / pow2 ind % 2;
-      (==) { limb_get_ith_bit_lemma a ind }
-      v (limb_get_ith_bit a ind);
-      (==) { }
-      1;
-      };
-    assert (v a / pow2 ind = 1) end;
-
-  calc (==) {
-    v a;
-    (==) { Math.Lemmas.euclidean_division_definition (v a) (pow2 (ind + 1)) }
-    v a % pow2 (ind + 1) + v a / pow2 (ind + 1) * pow2 (ind + 1);
-    (==) { }
-    v a % pow2 (ind + 1);
-    };
-  assert (v a < pow2 (ind + 1));
-
-  calc (==) {
-    v a;
-    (==) { Math.Lemmas.euclidean_division_definition (v a) (pow2 ind) }
-    v a % pow2 ind + v a / pow2 ind * pow2 ind;
-    (==) { }
-    v a % pow2 ind + pow2 ind;
-    };
-  assert (pow2 ind <= v a)
-
-
-val bn_get_num_bits: #t:limb_t -> #len:size_pos{bits t * len <= max_size_t} -> b:lbignum t len -> size_nat
-let bn_get_num_bits #t #len b =
-  let ind = bn_leading_zero_index #t #len b in
-  let last_bits = limb_leading_zero_index b.[ind] in
-  bits t * ind + last_bits
-
-
-val bn_get_num_bits_lemma_aux: d:pos -> ind:size_nat -> bs:size_nat -> a:nat -> b:nat -> Lemma
-  (requires
-    pow2 bs <= b /\ b < pow2 (bs + 1) /\ a < pow2 (d * ind))
-  (ensures
-    pow2 (d * ind + bs) <= a + pow2 (d * ind) * b /\
-    a + pow2 (d * ind) * b < pow2 (d * ind + bs + 1))
-
-let bn_get_num_bits_lemma_aux d ind bs a b =
-  calc (>=) {
-    a + pow2 (d * ind) * b;
-    (>=) { }
-    pow2 (d * ind) * b;
-    (>=) { }
-    pow2 (d * ind) * pow2 bs;
-    (==) { Math.Lemmas.pow2_plus (d * ind) bs }
-    pow2 (d * ind + bs);
-  };
-  assert (pow2 (d * ind + bs) <= a + pow2 (d * ind) * b);
-
-  calc (<=) {
-    a + pow2 (d * ind) * b;
-    (<=) { }
-    pow2 (d * ind) - 1 + pow2 (d * ind) * b;
-    (<=) { }
-    pow2 (d * ind) - 1 + pow2 (d * ind) * (pow2 (bs + 1) - 1);
-    (==) { Math.Lemmas.distributivity_sub_right (pow2 (d * ind)) (pow2 (bs + 1)) 1 }
-    pow2 (d * ind) * pow2 (bs + 1) - 1;
-    (==) { Math.Lemmas.pow2_plus (d * ind) (bs + 1) }
-    pow2 (d * ind + bs + 1) - 1;
-    };
-  assert (a + pow2 (d * ind) * b < pow2 (d * ind + bs + 1))
-
-
-val bn_get_num_bits_lemma: #t:limb_t -> #len:size_pos{bits t * len <= max_size_t} -> b:lbignum t len -> Lemma
-  (requires 0 < bn_v b)
-  (ensures (let bs = bn_get_num_bits b in
-    bs <= bits t * len /\ blocks (bs + 1) (bits t) <= len /\
-    pow2 bs <= bn_v b /\ bn_v b < pow2 (bs + 1)))
-
-let bn_get_num_bits_lemma #t #len b =
-  let ind = bn_leading_zero_index #t #len b in
-  bn_leading_zero_index_lemma b;
-  bn_leading_zero_index_eval_lemma b ind;
-  assert (bn_v b == bn_v (slice b 0 ind) + pow2 (bits t * ind) * v b.[ind]);
-  let bs = limb_leading_zero_index b.[ind] in
-  if ind = 0 then begin
-    bn_eval0 (slice b 0 ind);
-    assert_norm (pow2 0 = 1);
-    assert (bn_v b == v b.[ind]);
-    assert (v b.[ind] > 0);
-    () end;
-  assert (v b.[ind] > 0);
-  limb_leading_zero_index_lemma b.[ind];
-  limb_leading_zero_index_eval_lemma b.[ind] bs;
-  assert (pow2 bs <= v b.[ind] /\ v b.[ind] < pow2 (bs + 1));
-
-  bn_eval_bound (slice b 0 ind) ind;
-  bn_get_num_bits_lemma_aux (bits t) ind bs (bn_v (slice b 0 ind)) (v b.[ind])
-
-
-// val limb_get_num_bits_f: i:nat{i < 6} -> tuple2 uint64 pos -> tuple2 uint64 pos
-// let limb_get_num_bits_f i (l, bits) =
-//   assert_norm (pow2 5 = 32);
-//   Math.Lemmas.pow2_le_compat 5 (5 - i);
-//   let half_t = pow2 (5 - i) in
-//   let x = l >>. size half_t in
-//   let mask = u64 0 -. x in
-//   let mask = u64 0 -. (mask >>. 63ul) in
-//   let bits = if v mask = 0 then bits else bits + half_t in
-//   let l = l ^. (mask &. (x ^. l)) in
-//   (l, bits)
-
-
-// val limb_get_num_bits: a:uint64 -> pos
-// let limb_get_num_bits a =
-//   let (l, bits) = Loops.repeati 6 limb_get_num_bits_f (a, 1) in
-//   bits
-
-// val limb_get_num_bits_f_lemma: i:nat{i < 6} -> lb:tuple2 uint64 pos -> Lemma
-//   (requires (let l, bits = lb in 0 < v l))
-//   (ensures  (let l, bits = lb in
-//     let l1, bits1 = limb_get_num_bits_f i (l, bits) in
-//     let half_t = pow2 (5 - i) in
-//     let x = v l / pow2 half_t in 0 < v l1 /\ 0 < bits1 /\
-//     (if x = 0 then l1 == l /\ bits1 == bits else v l1 == x /\ bits1 == bits + half_t)))
-
-// let limb_get_num_bits_f_lemma i (l, bits) =
-//   let l1, bits1 = limb_get_num_bits_f i (l, bits) in
-//   assert_norm (pow2 5 = 32);
-//   Math.Lemmas.pow2_le_compat 5 (5 - i);
-//   let half_t = pow2 (5 - i) in
-//   let x = l >>. size half_t in
-//   assert (v x == v l / pow2 half_t);
-//   let mask = u64 0 -. x in
-//   if v x = 0 then begin
-//     assert (v mask = 0);
-//     let mask = u64 0 -. (mask >>. 63ul) in
-//     assert (v mask = 0);
-//     assert (bits1 = bits);
-//     BB.mask_select_lemma1 mask x l;
-//     assert (v l1 == v l);
-//     () end
-//   else begin
-//     // assert (v mask == pow2 64 - v x);
-//     assert (v mask == (- v x) % pow2 64);
-//     let mask1 = u64 0 -. (mask >>. 63ul) in
-//     assert (v mask1 = (- v mask / pow2 63) % pow2 64);
-//     calc (==) {
-//       (- v mask / pow2 63) % pow2 64;
-//       (==) { Math.Lemmas.lemma_mod_sub_1 (v mask / pow2 63) (pow2 64) }
-//       pow2 64 - (v mask / pow2 63) % pow2 64;
-//       (==) { Math.Lemmas.modulo_division_lemma (v mask) (pow2 63) (pow2 64) }
-//       pow2 64 - (v mask % (pow2 64 * pow2 63)) / pow2 63;
-//       (==) { Math.Lemmas.pow2_plus 64 63; Math.Lemmas.small_mod (v mask) (pow2 127) }
-//       pow2 64 - v mask / pow2 63;
-//       (==) { }
-//       pow2 64 - 1;
-//       };
-//     assert (v mask1 = v (ones U64 SEC));
-//     assert (bits1 = bits + half_t);
-//     BB.mask_select_lemma1 mask1 x l;
-//     assert (v l1 == v x);
-//     () end
-
-
-// val limb_get_num_bits_lemma_step: l1:pos -> i:pos{i <= 6} -> bits1:pos -> Lemma
-//   (let half_t = pow2 (6 - i) in
-//    let x = l1 / pow2 half_t in
-//    x * pow2 (bits1 + half_t - 1) <= l1 * pow2 (bits1 - 1))
-
-// let limb_get_num_bits_lemma_step l1 i bits1 =
-//   let half_t = pow2 (6 - i) in
-//   let x = l1 / pow2 half_t in
-
-//   calc (>=) {
-//     l1 * pow2 (bits1 - 1);
-//     (>=) { Math.Lemmas.multiply_fractions l1 (pow2 half_t) }
-//     x * pow2 half_t * pow2 (bits1 - 1);
-//     (==) { Math.Lemmas.paren_mul_right x (pow2 half_t) (pow2 (bits1 - 1));
-//       Math.Lemmas.pow2_plus half_t (bits1 - 1) }
-//     x * pow2 (bits1 + half_t - 1);
-//   }
-
-
-// val limb_get_num_bits_lemma_loop: a:uint64{0 < v a} -> i:nat{i <= 6} -> Lemma
-//   (let (l, bits) = Loops.repeati i limb_get_num_bits_f (a, 1) in
-//    let half_t = pow2 (6 - i) in
-//    v l < pow2 half_t /\ 0 < v l /\
-//    v l * pow2 (bits - 1) <= v a)
-
-// let rec limb_get_num_bits_lemma_loop a i =
-//   let (l, bits) = Loops.repeati i limb_get_num_bits_f (a, 1) in
-//   if i = 0 then begin
-//     Loops.eq_repeati0 i limb_get_num_bits_f (a, 1);
-//     assert_norm (pow2 0 = 1);
-//     assert_norm (pow2 1 = 2);
-//     assert_norm (pow2 6 = 64);
-//     () end
-//   else begin
-//     let (l1, bits1) = Loops.repeati (i - 1) limb_get_num_bits_f (a, 1) in
-//     Loops.unfold_repeati i limb_get_num_bits_f (a, 1) (i - 1);
-//     assert ((l, bits) == limb_get_num_bits_f (i - 1) (l1, bits1));
-//     limb_get_num_bits_lemma_loop a (i - 1);
-//     assert (v l1 * pow2 (bits1 - 1) <= v a /\ v l1 < pow2 (pow2 (7 - i)) /\ 0 < v l1 /\ 0 < bits1);
-//     limb_get_num_bits_f_lemma (i - 1) (l1, bits1);
-//     let half_t = pow2 (6 - i) in
-//     let x = v l1 / pow2 half_t in
-//     assert (if x = 0 then l == l1 /\ bits == bits1 else v l == x /\ bits == bits1 + half_t);
-//     assert (v l1 == x * pow2 half_t + v l1 % pow2 half_t);
-
-//     if x = 0 then ()
-//     else begin
-//       assert (pow2 (bits - 1) == pow2 (bits1 + half_t - 1));
-//       Math.Lemmas.pow2_double_sum (6 - i);
-//       Math.Lemmas.lemma_div_lt_nat (v l1) (pow2 (7 - i)) (pow2 (6 - i));
-//       assert (v l < pow2 half_t);
-//       limb_get_num_bits_lemma_step (v l1) i bits1;
-//       assert (v l * pow2 (bits1 + half_t - 1) <= v a);
-//     () end;
-
-//     () end
-
-
-// val limb_get_num_bits_lemma: a:uint64{v a > 0} -> Lemma (pow2 (limb_get_num_bits a - 1) <= v a)
-// let limb_get_num_bits_lemma a =
-//   let bits = limb_get_num_bits a in
-//   assert_norm (pow2 0 = 1);
-//   assert_norm (pow2 1 = 2);
-//   let (l, bits) = Loops.repeati 6 limb_get_num_bits_f (a, 1) in
-//   limb_get_num_bits_lemma_loop a 6;
-//   assert (0 < v l /\ v l < 2);
-//   assert (v l * pow2 (bits - 1) <= v a);
-//   assert (v l = 1)
+let bn_low_bound_bits_lemma #t #len b =
+  let ind = bn_get_top_index #t #len b in
+  bn_get_top_index_lemma #t #len b;
+  bn_get_top_index_eval_lemma #t #len b ind;
+  assert (pow2 (bn_low_bound_bits b) <= bn_v b);
+  if ind = 0 then
+    assert_norm (pow2 0 = 1)
+  else
+    Math.Lemmas.pow2_multiplication_modulo_lemma_1 1 1 (bn_low_bound_bits b)
