code/bignum/Hacl.Bignum.Exponentiation.fsti
@@ -83,7 +83,8 @@ val bn_mod_exp_mont_ladder_precompr2: #t:limb_t -> k:BM.mont t -> bn_mod_exp_mon
 
 inline_for_extraction noextract
 let bn_mod_exp_st (t:limb_t) (len:BN.meta_len t) =
-    n:lbignum t len
+    nBits:size_t{v nBits / bits t < v len}
+  -> n:lbignum t len
   -> a:lbignum t len
   -> bBits:size_t{0 < v bBits /\ bits t * v (blocks bBits (size (bits t))) <= max_size_t}
   -> b:lbignum t (blocks bBits (size (bits t)))
@@ -93,7 +94,7 @@ let bn_mod_exp_st (t:limb_t) (len:BN.meta_len t) =
     live h n /\ live h a /\ live h b /\ live h res /\
     disjoint res a /\ disjoint res b /\ disjoint res n /\ disjoint n a)
   (ensures  fun h0 _ h1 -> modifies (loc res) h0 h1 /\
-    as_seq h1 res == S.bn_mod_exp (v len) (as_seq h0 n) (as_seq h0 a) (v bBits) (as_seq h0 b))
+    as_seq h1 res == S.bn_mod_exp (v len) (v nBits) (as_seq h0 n) (as_seq h0 a) (v bBits) (as_seq h0 b))
 
 
 // This version is fully run-time.
@@ -108,7 +109,8 @@ val bn_mod_exp:
 
 inline_for_extraction noextract
 let bn_mod_exp_mont_ladder_st (t:limb_t) (len:BN.meta_len t) =
-    n:lbignum t len
+    nBits:size_t{v nBits / bits t < v len}
+  -> n:lbignum t len
   -> a:lbignum t len
   -> bBits:size_t{0 < v bBits /\ bits t * v (blocks bBits (size (bits t))) <= max_size_t}
   -> b:lbignum t (blocks bBits (size (bits t)))
@@ -118,7 +120,7 @@ let bn_mod_exp_mont_ladder_st (t:limb_t) (len:BN.meta_len t) =
     live h n /\ live h a /\ live h b /\ live h res /\
     disjoint res a /\ disjoint res b /\ disjoint res n /\ disjoint n a)
   (ensures  fun h0 _ h1 -> modifies (loc res) h0 h1 /\
-    as_seq h1 res == S.bn_mod_exp_mont_ladder (v len) (as_seq h0 n) (as_seq h0 a) (v bBits) (as_seq h0 b))
+    as_seq h1 res == S.bn_mod_exp_mont_ladder (v len) (v nBits) (as_seq h0 n) (as_seq h0 a) (v bBits) (as_seq h0 b))
 
 // This version is fully run-time.
 // This function is constant-time on the exponent b.
