code/ffdhe/Hacl.Spec.FFDHE.Lemmas.fst
@@ -1,0 +1,104 @@
+module Hacl.Spec.FFDHE.Lemmas
+
+open FStar.Mul
+
+open Lib.IntTypes
+open Lib.Sequence
+open Lib.ByteSequence
+open Spec.FFDHE
+
+#set-options "--z3rlimit 50 --fuel 0 --ifuel 0"
+
+
+val ffdhe_p_lemma_len: a:ffdhe_alg -> Lemma
+ (let ffdhe_p = get_ffdhe_params a in
+  let p = Mk_ffdhe_params?.ffdhe_p ffdhe_p in
+  Seq.index p 0 == 0xffuy)
+
+let ffdhe_p_lemma_len a =
+  let ffdhe_p = get_ffdhe_params a in
+  let p = Mk_ffdhe_params?.ffdhe_p ffdhe_p in
+
+  allow_inversion ffdhe_alg;
+  match a with
+  | FFDHE2048 ->
+    assert (p == of_list list_ffdhe_p2048);
+    assert_norm (List.Tot.index list_ffdhe_p2048 0 == 0xffuy);
+    assert (Seq.index (Seq.seq_of_list list_ffdhe_p2048) 0 == 0xffuy)
+  | FFDHE3072 ->
+    assert (p == of_list list_ffdhe_p3072);
+    assert_norm (List.Tot.index list_ffdhe_p3072 0 == 0xffuy);
+    assert (Seq.index (Seq.seq_of_list list_ffdhe_p3072) 0 == 0xffuy)
+  | FFDHE4096 ->
+    assert (p == of_list list_ffdhe_p4096);
+    assert_norm (List.Tot.index list_ffdhe_p4096 0 == 0xffuy);
+    assert (Seq.index (Seq.seq_of_list list_ffdhe_p4096) 0 == 0xffuy)
+  | FFDHE6144 ->
+    assert (p == of_list list_ffdhe_p6144);
+    assert_norm (List.Tot.index list_ffdhe_p6144 0 == 0xffuy);
+    assert (Seq.index (Seq.seq_of_list list_ffdhe_p6144) 0 == 0xffuy)
+  | FFDHE8192 ->
+    assert (p == of_list list_ffdhe_p8192);
+    assert_norm (List.Tot.index list_ffdhe_p8192 0 == 0xffuy);
+    assert (Seq.index (Seq.seq_of_list list_ffdhe_p8192) 0 == 0xffuy)
+
+
+// the proof should be somehow simpler
+val pow2_lt_len: len:size_pos -> Lemma (pow2 (8 * len - 1) < pow2 (8 * (len - 1)) * (pow2 8 - 1))
+let pow2_lt_len len =
+  let a = pow2 (8 * len - 1) in
+  let b = pow2 (8 * (len - 1)) * (pow2 8 - 1) in
+  calc (==) {
+    b / a;
+    (==) { Math.Lemmas.pow2_plus (8 * len - 8) 7 }
+    b / (pow2 (8 * len - 8) * pow2 7);
+    (==) { Math.Lemmas.division_multiplication_lemma b (pow2 (8 * len - 8)) (pow2 7) }
+    b / pow2 (8 * len - 8) / pow2 7;
+    (==) { Math.Lemmas.cancel_mul_div (pow2 8 - 1) (pow2 (8 * len - 8)) }
+    (pow2 8 - 1) / pow2 7;
+    (==) { Math.Lemmas.pow2_plus 7 1 }
+    (pow2 7 * 2 - 1) / pow2 7;
+    (==) { }
+    1;
+    };
+  //  assert (b / a * a <= b);
+  //  assert (a <= b)
+
+  calc (>) {
+    pow2 (8 * len - 8) * (pow2 8 - 1) % pow2 (8 * len - 1);
+    (==) { Math.Lemmas.pow2_plus (8 * len - 8) 8 }
+    (pow2 (8 * len) - pow2 (8 * len - 8)) % pow2 (8 * len - 1);
+    (==) { Math.Lemmas.lemma_mod_plus_distr_l (pow2 (8 * len)) (- pow2 (8 * len - 8)) (pow2 (8 * len - 1)) }
+    (pow2 (8 * len) % pow2 (8 * len - 1) - pow2 (8 * len - 8)) % pow2 (8 * len - 1);
+    (==) { Math.Lemmas.pow2_multiplication_modulo_lemma_1 1 (8 * len - 1) (8 * len) }
+    (0 - pow2 (8 * len - 8)) % pow2 (8 * len - 1);
+    //(==) { Math.Lemmas.pow2_lt_compat (8 * len - 1) (8 * len - 8) }
+    //pow2 (8 * len - 1) - pow2 (8 * len - 8);
+    (>) { Math.Lemmas.pow2_lt_compat (8 * len - 1) (8 * len - 8) }
+    0;
+    };
+
+  assert (a < b)
+
+
+val ffdhe_p_bits_lemma: a:ffdhe_alg -> Lemma
+ (let ffdhe_p = get_ffdhe_params a in
+  let len = ffdhe_len a in
+  let p = Mk_ffdhe_params?.ffdhe_p ffdhe_p in
+  let p_n = nat_from_bytes_be p in
+  pow2 (8 * len - 1) < p_n)
+
+let ffdhe_p_bits_lemma a =
+  let ffdhe_p = get_ffdhe_params a in
+  let len = ffdhe_len a in
+  let p = Mk_ffdhe_params?.ffdhe_p ffdhe_p in
+  let p_n = nat_from_bytes_be p in
+
+  nat_from_intseq_be_slice_lemma p 1;
+  assert (p_n == nat_from_bytes_be (slice p 1 len) + pow2 (8 * (len - 1)) * nat_from_bytes_be (slice p 0 1));
+  nat_from_intseq_be_lemma0 (slice p 0 1);
+  assert (p_n == nat_from_bytes_be (slice p 1 len) + pow2 (8 * (len - 1)) * v p.[0]);
+  assert (pow2 (8 * (len - 1)) * v p.[0] <= p_n);
+  ffdhe_p_lemma_len a;
+  assert (pow2 (8 * (len - 1)) * (pow2 8 - 1) <= p_n);
+  pow2_lt_len len
